src/lib/poly/gemm/Kuiper.Poly.GEMM.TensorCore2D.fst
@@ -4,7 +4,7 @@ module Kuiper.Poly.GEMM.TensorCore2D
 
 open Kuiper
 #set-options "--ifuel 1 --initial_fuel 0 --max_fuel 1"
-#set-options "--z3rlimit 60"
+#set-options "--z3rlimit 120"
 
 open Kuiper.Approximates
 open Kuiper.Array.Vectorized { has_vec_cpy, chunk }
